crates/sui/src/sui_move/sui-natives.bpl
@@ -14,6 +14,10 @@ procedure {:inline 1} $2_address_from_u256(num: int) returns (res: int);
 // ==================================================================================
 // Native transfer
 
+const INVALID_ADDR: int;
+axiom INVALID_ADDR == -1;
+
+
 function {:inline} ownership_update<T>(m: $Memory T, id: int, v: T): $Memory T {
     $Memory(domain#$Memory(m)[id := true], contents#$Memory(m)[id := v])
 }
@@ -26,13 +30,11 @@ function {:inline} ownership_update<T>(m: $Memory T, id: int, v: T): $Memory T {
 // ----------------------------------------------------------------------------------
 // Native transfer implementation for object type `{{instance.suffix}}`
 
-
-
 procedure {:inline 1} $2_transfer_transfer_internal{{S}}(obj: {{T}}, recipient: int) {
     var id: int;
     var v: $2_prover_Ownership;
     id := $bytes#$2_object_ID($2_object_$id{{S}}(obj));
-    v := $2_prover_Ownership($1_option_spec_some'address'(recipient), 1);
+    v := $2_prover_Ownership(recipient, 1);
     $2_prover_Ownership_$memory := ownership_update($2_prover_Ownership_$memory, id, v);
 }
 
@@ -45,7 +47,7 @@ procedure {:inline 1} $2_transfer_share_object{{S}}(obj: {{T}}) {
     }
 
     id := $bytes#$2_object_ID($2_object_$id{{S}}(obj));
-    v := $2_prover_Ownership($1_option_Option'address'(EmptyVec()), 2);
+    v := $2_prover_Ownership(INVALID_ADDR, 2);
     $2_prover_Ownership_$memory := ownership_update($2_prover_Ownership_$memory, id, v);
 }
 
@@ -58,7 +60,7 @@ procedure {:inline 1} $2_transfer_freeze_object{{S}}(obj: {{T}}) {
     }
 
     id := $bytes#$2_object_ID($2_object_$id{{S}}(obj));
-    v := $2_prover_Ownership($1_option_Option'address'(EmptyVec()), 3);
+    v := $2_prover_Ownership(INVALID_ADDR, 3);
     $2_prover_Ownership_$memory := ownership_update($2_prover_Ownership_$memory, id, v);
 }
 
