crates/sui-framework/docs/dynamic_field.md
@@ -168,13 +168,16 @@ Aborts with <code><a href="dynamic_field.md#0x2_dynamic_field_EFieldAlreadyExist
 
 <pre><code><b>pragma</b> opaque;
 <b>aborts_if</b> [abstract] sui::prover::uid_has_field(<a href="object.md#0x2_object">object</a>.id.bytes, name);
-<b>ensures</b> [abstract] <a href="object.md#0x2_object">object</a>.id == <b>old</b>(<a href="object.md#0x2_object">object</a>.id);
-<b>ensures</b> [abstract] <b>global</b>&lt;sui::prover::DynamicFields&lt;Name&gt;&gt;(<a href="object.md#0x2_object">object</a>.id.bytes).names
-    == concat(
-        <b>old</b>(<b>global</b>&lt;sui::prover::DynamicFields&lt;Name&gt;&gt;(<a href="object.md#0x2_object">object</a>.id.bytes)).names,
-        vec(name)
-    );
-<b>ensures</b> [abstract] len(<b>global</b>&lt;sui::prover::DynamicFields&lt;Name&gt;&gt;(<a href="object.md#0x2_object">object</a>.id.bytes).names) == len(<b>old</b>(<b>global</b>&lt;sui::prover::DynamicFields&lt;Name&gt;&gt;(<a href="object.md#0x2_object">object</a>.id.bytes).names)) + 1;
+<b>modifies</b> [abstract] <b>global</b>&lt;sui::prover::DynamicFields&lt;Name&gt;&gt;(<a href="object.md#0x2_object">object</a>.id.bytes);
+<b>ensures</b> [abstract] <a href="object.md#0x2_object">object</a> == <b>old</b>(<a href="object.md#0x2_object">object</a>);
+<b>ensures</b> [abstract] <b>exists</b>&lt;sui::prover::DynamicFields&lt;Name&gt;&gt;(<a href="object.md#0x2_object">object</a>.id.bytes);
+<b>ensures</b> [abstract] (!<b>old</b>(<b>exists</b>&lt;sui::prover::DynamicFields&lt;Name&gt;&gt;(<a href="object.md#0x2_object">object</a>.id.bytes)))
+    ==&gt; <b>global</b>&lt;sui::prover::DynamicFields&lt;Name&gt;&gt;(<a href="object.md#0x2_object">object</a>.id.bytes).names == vec(name);
+<b>ensures</b> [abstract] <b>old</b>(<b>exists</b>&lt;sui::prover::DynamicFields&lt;Name&gt;&gt;(<a href="object.md#0x2_object">object</a>.id.bytes))
+    ==&gt; <b>global</b>&lt;sui::prover::DynamicFields&lt;Name&gt;&gt;(<a href="object.md#0x2_object">object</a>.id.bytes).names == concat(
+            <b>old</b>(<b>global</b>&lt;sui::prover::DynamicFields&lt;Name&gt;&gt;(<a href="object.md#0x2_object">object</a>.id.bytes).names),
+            vec(name)
+        );
 </code></pre>
 
 
@@ -318,12 +321,12 @@ type.
 
 <pre><code><b>pragma</b> opaque;
 <b>aborts_if</b> [abstract] !sui::prover::uid_has_field(<a href="object.md#0x2_object">object</a>.id.bytes, name);
+<b>modifies</b> [abstract] <b>global</b>&lt;sui::prover::DynamicFields&lt;Name&gt;&gt;(<a href="object.md#0x2_object">object</a>.id.bytes);
 <b>ensures</b> [abstract] <a href="object.md#0x2_object">object</a>.id == <b>old</b>(<a href="object.md#0x2_object">object</a>.id);
+<b>ensures</b> [abstract] <b>exists</b>&lt;sui::prover::DynamicFields&lt;Name&gt;&gt;(<a href="object.md#0x2_object">object</a>.id.bytes);
 <b>ensures</b> [abstract] sui::prover::vec_remove(<b>global</b>&lt;sui::prover::DynamicFields&lt;Name&gt;&gt;(<a href="object.md#0x2_object">object</a>.id.bytes).names,
-    index_of(<b>global</b>&lt;sui::prover::DynamicFields&lt;Name&gt;&gt;(<a href="object.md#0x2_object">object</a>.id.bytes).names, name),
-    0) ==
+    index_of(<b>global</b>&lt;sui::prover::DynamicFields&lt;Name&gt;&gt;(<a href="object.md#0x2_object">object</a>.id.bytes).names, name), 0) ==
       <b>old</b>(<b>global</b>&lt;sui::prover::DynamicFields&lt;Name&gt;&gt;(<a href="object.md#0x2_object">object</a>.id.bytes).names);
-<b>ensures</b> [abstract] len(<b>global</b>&lt;sui::prover::DynamicFields&lt;Name&gt;&gt;(<a href="object.md#0x2_object">object</a>.id.bytes).names) == len(<b>old</b>(<b>global</b>&lt;sui::prover::DynamicFields&lt;Name&gt;&gt;(<a href="object.md#0x2_object">object</a>.id.bytes).names)) - 1;
 </code></pre>
 
 
