crates/sui-framework/docs/prover.md
@@ -7,12 +7,12 @@
 
 -  [Resource `Ownership`](#0x2_prover_Ownership)
 -  [Resource `DynamicFields`](#0x2_prover_DynamicFields)
+-  [Resource `DynamicFieldContainment`](#0x2_prover_DynamicFieldContainment)
 -  [Constants](#@Constants_0)
 -  [Module Specification](#@Module_Specification_1)
 
 
-<pre><code><b>use</b> <a href="">0x1::option</a>;
-</code></pre>
+<pre><code></code></pre>
 
 
 
@@ -20,6 +20,7 @@
 
 ## Resource `Ownership`
 
+Ownership information for a given object (stored at the object's address)
 
 
 <pre><code><b>struct</b> <a href="prover.md#0x2_prover_Ownership">Ownership</a> <b>has</b> key
@@ -33,7 +34,7 @@
 
 <dl>
 <dt>
-<code>owner: <a href="_Option">option::Option</a>&lt;<b>address</b>&gt;</code>
+<code>owner: <b>address</b></code>
 </dt>
 <dd>
 
@@ -53,6 +54,8 @@
 
 ## Resource `DynamicFields`
 
+List of fields with a given name type of an object containing fields (stored at the
+containing object's address)
 
 
 <pre><code><b>struct</b> <a href="prover.md#0x2_prover_DynamicFields">DynamicFields</a>&lt;K: <b>copy</b>, drop, store&gt; <b>has</b> key
@@ -67,6 +70,35 @@
 <dl>
 <dt>
 <code>names: <a href="">vector</a>&lt;K&gt;</code>
+</dt>
+<dd>
+
+</dd>
+</dl>
+
+
+</details>
+
+<a name="0x2_prover_DynamicFieldContainment"></a>
+
+## Resource `DynamicFieldContainment`
+
+Information about which object contains a given object field (stored at the field object's
+address).
+
+
+<pre><code><b>struct</b> <a href="prover.md#0x2_prover_DynamicFieldContainment">DynamicFieldContainment</a> <b>has</b> key
+</code></pre>
+
+
+
+<details>
+<summary>Fields</summary>
+
+
+<dl>
+<dt>
+<code>container: <b>address</b></code>
 </dt>
 <dd>
 
@@ -112,6 +144,7 @@
 
 ## Module Specification
 
+Verifies if a given object it owned.
 
 
 <a name="0x2_prover_owned"></a>
@@ -120,12 +153,12 @@
 <pre><code><b>fun</b> <a href="prover.md#0x2_prover_owned">owned</a>&lt;T: key&gt;(obj: T): bool {
    <b>let</b> addr = <a href="object.md#0x2_object_id">object::id</a>(obj).bytes;
    <b>exists</b>&lt;<a href="prover.md#0x2_prover_Ownership">Ownership</a>&gt;(addr) &&
-   <a href="_is_some">option::is_some</a>(<b>global</b>&lt;<a href="prover.md#0x2_prover_Ownership">Ownership</a>&gt;(addr).owner) &&
    <b>global</b>&lt;<a href="prover.md#0x2_prover_Ownership">Ownership</a>&gt;(addr).status == <a href="prover.md#0x2_prover_OWNED">OWNED</a>
 }
 </code></pre>
 
 
+Verifies if a given object is owned.
 
 
 <a name="0x2_prover_owned_by"></a>
@@ -134,12 +167,13 @@
 <pre><code><b>fun</b> <a href="prover.md#0x2_prover_owned_by">owned_by</a>&lt;T: key&gt;(obj: T, owner: <b>address</b>): bool {
    <b>let</b> addr = <a href="object.md#0x2_object_id">object::id</a>(obj).bytes;
    <b>exists</b>&lt;<a href="prover.md#0x2_prover_Ownership">Ownership</a>&gt;(addr) &&
-   <b>global</b>&lt;<a href="prover.md#0x2_prover_Ownership">Ownership</a>&gt;(addr).owner == <a href="_spec_some">option::spec_some</a>(owner) &&
-   <b>global</b>&lt;<a href="prover.md#0x2_prover_Ownership">Ownership</a>&gt;(addr).status == <a href="prover.md#0x2_prover_OWNED">OWNED</a>
+   <b>global</b>&lt;<a href="prover.md#0x2_prover_Ownership">Ownership</a>&gt;(addr).status == <a href="prover.md#0x2_prover_OWNED">OWNED</a> &&
+   <b>global</b>&lt;<a href="prover.md#0x2_prover_Ownership">Ownership</a>&gt;(addr).owner == owner
 }
 </code></pre>
 
 
+Verifies if a given object is shared.
 
 
 <a name="0x2_prover_shared"></a>
@@ -148,12 +182,12 @@
 <pre><code><b>fun</b> <a href="prover.md#0x2_prover_shared">shared</a>&lt;T: key&gt;(obj: T): bool {
    <b>let</b> addr = <a href="object.md#0x2_object_id">object::id</a>(obj).bytes;
    <b>exists</b>&lt;<a href="prover.md#0x2_prover_Ownership">Ownership</a>&gt;(addr) &&
-   <a href="_is_none">option::is_none</a>(<b>global</b>&lt;<a href="prover.md#0x2_prover_Ownership">Ownership</a>&gt;(addr).owner) &&
    <b>global</b>&lt;<a href="prover.md#0x2_prover_Ownership">Ownership</a>&gt;(addr).status == <a href="prover.md#0x2_prover_SHARED">SHARED</a>
 }
 </code></pre>
 
 
+Verifies if a given object is immutable.
 
 
 <a name="0x2_prover_immutable"></a>
@@ -162,12 +196,12 @@
 <pre><code><b>fun</b> <a href="prover.md#0x2_prover_immutable">immutable</a>&lt;T: key&gt;(obj: T): bool {
    <b>let</b> addr = <a href="object.md#0x2_object_id">object::id</a>(obj).bytes;
    <b>exists</b>&lt;<a href="prover.md#0x2_prover_Ownership">Ownership</a>&gt;(addr) &&
-   <a href="_is_none">option::is_none</a>(<b>global</b>&lt;<a href="prover.md#0x2_prover_Ownership">Ownership</a>&gt;(addr).owner) &&
    <b>global</b>&lt;<a href="prover.md#0x2_prover_Ownership">Ownership</a>&gt;(addr).status == <a href="prover.md#0x2_prover_IMMUTABLE">IMMUTABLE</a>
 }
 </code></pre>
 
 
+Verifies if a given object has field with a given name.
 
 
 <a name="0x2_prover_has_field"></a>
@@ -180,6 +214,7 @@
 </code></pre>
 
 
+Returns number of K-type fields of a given object.
 
 
 <a name="0x2_prover_num_fields"></a>
